Surface/Metatheory.lean
@@ -1,4 +1,0 @@
-import Surface.Metatheory.Rename
-import Surface.Metatheory.Substitution
-import Surface.Metatheory.GlobalWf
-import Surface.Metatheory.Inversion
