Translation/Global.lean
@@ -9,52 +9,80 @@ import Translation.Term
 
 
 
+inductive Translation.GlobalWf : Surface.GlobalEnv -> Core.GlobalEnv -> Surface.Global -> Prop where
+| data {ctors : Vect n (String × Surface.Ty)} {G : Surface.GlobalEnv}{G' : Core.GlobalEnv}:
+  (∀ i y T, ctors i = (y, T) ->
+    (Surface.Global.data x K Vect.nil :: G)&[] ⊢s T : `★
+    ∧ Surface.ValidCtor x T
+    ∧ x ≠ y
+    ∧ Surface.lookup y G = none) ->
+  (∀ i j, (ctors i).1 ≠ (ctors j).1) ->
+  Surface.lookup x G = none ->
+  GlobalWf G G' (Surface.Global.data x K ctors)
+| defn :
+  Surface.lookup x G = none ->
+  G&[] ⊢s T : `★ ->
+  Surface.Term.Elab G G' .chk [] [] t T t' ->
+  GlobalWf G G' (Surface.Global.defn x T t)
+| classDecl :
+  Surface.lookup s G = none ->
+  Surface.ValidOpenKind K ->
+  (∀ i j, (ms i).1 ≠ (ms j).1) ->
+  (∀ i y T, ms i = (y, T) ->
+    (Surface.Global.classDecl s K Vect.nil :: G)&[] ⊢s T : `★
+    ∧ Surface.ValidClassMethodTy s T
+    ∧ s ≠ y
+    ∧ Surface.lookup y G = none) ->
+  GlobalWf G G' (Surface.Global.classDecl s K ms)
+| instDecl :
+  Surface.ValidClassInstTy C T ->
+  -- TODO: Do Non-overlapping check here
+  Surface.lookup C G = some (.opent C K ms') ->
+  -- TODO: check for method types
+  GlobalWf G G' (.instDecl T ms)
 
 
-def Surface.Ty.translate_ctors (ctors : Vect n (String × Surface.Ty)) : (Vect n (String × Core.Ty)) :=
-  (λ (x, ty) => (x , ty.translate)) <$> ctors
-
-
--- @[simp]
--- def Surface.Global.translate (G : Surface.GlobalEnv) (G' : Core.GlobalEnv) : Global -> Option Core.Global
--- | .data (n := n) x K ctors =>
---   let ctors' := Ty.translate_ctors ctors
---   Core.Global.data n x K.translate ctors'
--- | instDecl x t => do
---   let T <- Surface.lookup_type G x
---   let t' <- t.type_chk_translate G G' [] [] T
---   return .inst x t'
--- | defn x T t => do
---   let t' <- t.type_chk_translate G G' [] [] T
---   return .defn x T.translate t'
--- | openm x T => return .openm x T.translate
--- | opent x K => return .opent x K.translate
-
-
-
--- @[simp]
--- def Surface.GlobalEnv.translate : Surface.GlobalEnv -> Option (Core.GlobalEnv)
--- | [] => return []
--- | .cons g gs => do
---   let gs' <- Surface.GlobalEnv.translate gs
---   let g' <- g.translate gs gs'
---   return (g' :: gs')
-
--- def Surface.Entry.translate : Surface.Entry -> Option
 
 inductive Surface.Global.Elab : Surface.GlobalEnv -> Core.GlobalEnv -> Prop
 | nil : Surface.Global.Elab [] []
+
 | defn :
   Surface.Global.Elab G G' ->
+
+  Surface.lookup x G = none ->
+  G&[] ⊢s T : `★ ->
   Surface.Term.Elab G G' .chk [] [] t T t' ->
+
   Surface.Global.Elab (.cons (.defn x T t) G) ((.defn x (T.translate) t') :: G')
+
 | data {n : Nat} {ctors : Vect n (String × Ty)} {ctors' : Vect n (String × Core.Ty)} :
   Surface.Global.Elab G G' ->
+
+  (∀ i y T, ctors i = (y, T) ->
+    (Surface.Global.data x K Vect.nil :: G)&[] ⊢s T : `★
+    ∧ Surface.ValidCtor x T
+    ∧ x ≠ y
+    ∧ Surface.lookup y G = none) ->
+  (∀ i j, (ctors i).1 ≠ (ctors j).1) ->
+  Surface.lookup x G = none ->
+
   ctors' = (λ i => ((ctors i).1 , (ctors i).2.translate)) ->
+
   Surface.Global.Elab (.cons (.data (n := n) x K ctors) G) (.cons (.data n x K.translate ctors') G')
-| classDecl {n : Nat} {ms : Vect n (String × Ty)} {ms' : Vect n Core.Global}:
+
+| classDecl {n : Nat} {ms : Vect n (String × Ty)} {ms' : Vect n Core.Global} :
   Surface.Global.Elab G G' ->
+
+  Surface.lookup x G = none ->
+  Surface.ValidOpenKind K ->
+  (∀ i j, (ms i).1 ≠ (ms j).1) ->
+  (∀ i y T, ms i = (y, T) ->
+    (Surface.Global.classDecl x K Vect.nil :: G)&[] ⊢s T : `★
+    ∧ Surface.ValidClassMethodTy x T
+    ∧ x ≠ y
+    ∧ Surface.lookup y G = none) ->
   ms' = (λ i => Core.Global.openm (ms i).1 (ms i).2.translate) ->
+
   Surface.Global.Elab ((.classDecl x K ms) :: G) (ms'.to_list ++ (Core.Global.opent x K.translate :: G'))
 
 
