Translation/Global/Lemmas.lean
@@ -8,76 +8,6 @@ import Translation.Ty.Lemmas
 import Translation.Term.Lemmas
 import Translation.Global
 import Core.Metatheory.Determined.Semantic
--- theorem Translation.Ty.ValidCtor :
---   Surface.ValidCtor x T -> Core.ValidCtor x ⟦T⟧ := by
--- intro h; induction h <;> simp at *
--- case base h1 h2 =>
---   replace lem := Translation.Ty.Spine h2 rfl
---   rcases lem with ⟨_, lem⟩
---   constructor; assumption
--- case all ih => apply Core.ValidCtor.all ih
--- case arrow ih => apply Core.ValidCtor.arrow ih
-
--- theorem Translation.Global.empty_data_wkn {G : Surface.GlobalEnv} {G' : Core.GlobalEnv} (x : String) (K : Surface.Kind) :
---   G.translate = G' ->
---   Surface.GlobalEnv.translate (.data x K Vect.nil :: G) = (.data 0 x ⟦K⟧ Vect.nil :: G') := by
--- intro h; simp [Surface.GlobalEnv.translate]; exact h
-
--- theorem Surface.GlobalEnvWf.empty_data_wkn x K :
---   ⊢s G -> lookup x G = none ->
---   ⊢s (Surface.Global.data x K Vect.nil :: G) := by
---  intro wf lk; apply ListGlobalWf.cons
---  · apply GlobalWf.data <;> try simp at *
---    apply Vect.nil
---    apply lk
---  · assumption
-
--- theorem Translation.GlobalWf.sound {G : Surface.GlobalEnv} {g : Surface.Global}:
---   ⊢s G ->
---   Surface.GlobalWf G g ->
---   G.translate = G' ->
---   ⊢ G' ->
---  ∃ g',
---     g.translate = g'  ∧
---     Core.GlobalWf G' g' := by
--- intro wf h1 h2 h3; induction g <;> simp at *
--- cases h1
--- case _ n x K ctors cns lk cnsdef ctor_trans =>
--- let ctors' : Vect n (String × Core.Ty) := Surface.Ty.translate_ctors ctors
--- apply Core.GlobalWf.data
--- · intro i y T e;
---   replace ctor_trans := ctor_trans i (ctors i).fst (ctors i).snd rfl;
---   rcases ctor_trans with ⟨k1, k2, k3, k4⟩
---   rcases e with ⟨e1, e2⟩;
---   have lemG := Translation.Global.empty_data_wkn x K h2
---   have wfG := Surface.GlobalEnvWf.empty_data_wkn x K wf lk
---   have lem := Translation.Ty.sound wfG (G := .data x K Vect.nil :: G) ⟨k1,lemG, rfl⟩
---   apply And.intro
---   · rcases lem with ⟨K', T', e1, e2, e3⟩;
---     simp at e1; subst e1; subst e2; simp [Surface.KindEnv.translate] at e3; apply e3
---   · apply And.intro
---     · apply Translation.Ty.ValidCtor k2
---     · apply And.intro; assumption
---       apply Translation.GlobalEnv.lookup_none_sound _ h2 k4
--- · assumption
--- · apply Translation.GlobalEnv.lookup_none_sound _ h2 lk
-
-
--- theorem Translation.GlobalEnv.wf_sound {G : Surface.GlobalEnv} :
---   ⊢s G ->
---   ⊢ G.translate
--- := by
--- intro wf
--- induction G <;> simp at *
--- case _ => apply Core.ListGlobalWf.nil
--- case _ g gs ih =>
--- cases wf; case _ wfgs wfg =>
--- replace ih := ih wfgs
--- have lem := Translation.GlobalWf.sound wfgs  wfg rfl ih
--- rcases lem with ⟨g', lem1, lem2⟩; subst g'
--- cases g; simp [Surface.Global.translate] at lem2;
--- apply Core.ListGlobalWf.cons _ ih
--- simp; apply lem2
 
 theorem Translation.ValidOpenKind.Sound {K : Surface.Kind}:
   Surface.ValidOpenKind K -> Core.ValidOpenKind K.translate := by
@@ -87,72 +17,104 @@ theorem Translation.ValidOpenKind.Sound {K : Surface.Kind}:
   constructor; assumption
 
 theorem Surface.Global.Elab.sound :
-  ⊢s G ->
   G -↪ G' ->
   ⊢ G' ∧ Core.Global.Determined G' := by
-intro wf h
+intro h
 induction h
 case nil =>
   apply And.intro
   · apply Core.ListGlobalWf.nil;
   · simp [Core.Global.Determined, Core.Determined.openm, Core.Determined.defn, Core.lookup];
-case defn t T t' x j0 jdef ih =>
-  cases wf; case _ wfh wftl =>
-  replace ih := ih wfh
-  cases wftl; case _ lk j1 j2 =>
+case defn x T t t' j0 lk j1 j2 ih =>
   replace j1 := Translation.Ty.sound j1 j0 rfl
-  rcases j1 with ⟨K, T', e1, e2, j1⟩
-  subst e1; cases e2; simp at j1;
-  replace j2 := Translation.Term.Sound2 j0 jdef [] [] rfl rfl
+  rcases j1 with ⟨K, T', e1, e2, j1⟩; subst e1; subst e2
+  replace j2 := Translation.Term.Sound j0 j2 [] [] rfl rfl
   apply And.intro
   · apply Core.ListGlobalWf.cons _ ih.1
     apply Core.GlobalWf.defn j1 j2.2
-    · apply Translation.GlobalEnv.lookup_none_sound x j0 lk
+    apply Translation.GlobalEnv.lookup_none_sound x j0 lk
   · sorry
-case data wf =>
-  cases wf; case _ wfh wftl =>
-  replace wf := wf wfh
-  cases wftl; case _ G G' x K n ctors _ j0 ctors'def lk h1 h2 =>
+
+case data G G' x K n ctors ctors' j0 h1 h2 h3 ctors'def ih  =>
   apply And.intro
-  · apply Core.ListGlobalWf.cons _ wf.1;
+  · apply Core.ListGlobalWf.cons _ ih.1;
     apply Core.GlobalWf.data
-    · intro i y T h1;
-      simp [ctors'def] at h1; rcases h1 with ⟨h1a, h1b⟩
-      replace h2 := h2 i (ctors i).fst (ctors i).snd rfl;
-      rcases h2 with ⟨h2a, h2b, h2c, h2d⟩
+    · intro i y T h1';
+      simp [ctors'def] at h1'; rcases h1' with ⟨h1a, h1b⟩
+      replace h1 := h1 i (ctors i).fst (ctors i).snd rfl;
+      rcases h1 with ⟨h2a, h2b, h2c, h2d⟩
       have wkn_j0 : Elab (.data x K Vect.nil :: G) (.cons (.data 0 x K.translate Vect.nil) G') := by
-        apply Elab.data j0; simp
+        apply Elab.data j0; simp; simp; apply h3; simp
+
       replace h2a := Translation.Ty.sound h2a wkn_j0 rfl
       rcases h2a with ⟨_, _, e1, e2, h2a⟩; subst e1; subst e2
       subst y; subst T
       replace h2d := Translation.GlobalEnv.lookup_none_sound (ctors i).fst j0 h2d
       grind
-    · intro i j; simp [ctors'def]; apply h1
-    · apply Translation.GlobalEnv.lookup_none_sound x j0 lk
+    · intro i j; simp [ctors'def]; apply h2
+    · apply Translation.GlobalEnv.lookup_none_sound x j0 h3
   · sorry
-case classDecl wf =>
-  cases wf; case _ wfh wftl =>
-  replace wf := wf wfh
-  cases wftl; case _ G G' x K n ms ms' j0 ms'def lk h1 h2 h3 =>
+case classDecl G G' x K n ms ms' j0 h1 h2 h3 h4 ms'def ih =>
   have wkn_j0 : Elab (.cons (.classDecl x K Vect.nil) G) (.cons (.opent x K.translate) G') := by
-    apply Elab.classDecl (x := x) (K := K) (ms := Vect.nil) (ms' := Vect.nil) j0; simp
+    apply Elab.classDecl (x := x) (K := K) (ms := Vect.nil) (ms' := Vect.nil) _ _
+    apply h2
+    simp
+    simp
+    simp
+    apply j0
+    apply h1
   apply And.intro
-  · simp;
-    revert ms'; revert ms; intro ms; apply ms.induction
-    case _ =>
+  · simp; revert ms'; revert ms; intro ms
+    apply ms.induction
+    case nil =>
       simp; intro ms'
-      apply Core.ListGlobalWf.cons _ wf.1;
+      apply Core.ListGlobalWf.cons _ ih.1
       apply Core.GlobalWf.opent
-      apply Translation.ValidOpenKind.Sound h1
-      apply Translation.GlobalEnv.lookup_none_sound x j0 lk
-    case _ =>
-      simp; intro n mthname mthTy ms ih1 ih2 ih3
-      generalize mdef : (Vect.fold [] List.cons fun i =>
-        Core.Global.openm ( Vect.cons (mthname, mthTy) ms i).fst ⟦(Vect.cons (mthname, mthTy) ms i).snd⟧) = ms' at *
+      apply Translation.ValidOpenKind.Sound h2
+      apply Translation.GlobalEnv.lookup_none_sound x j0 h1
+    case cons =>
+      intro n hd tl h1 h2 h3 ms' ms'def
+      replace ms'def := Vect.map_cons ms'def (f := λ (x : String × Ty) => Core.Global.openm x.1 x.2.translate)
+      rw[ms'def]; simp;
+      apply Core.ListGlobalWf.cons _ _
+      · sorry
+      · apply h1
+        sorry
+        sorry
+        rfl
 
 
-    --   intro n hd tl wftl
-    --   simp; apply Core.ListGlobalWf.cons _ wftl;
+    -- apply Core.ListGlobalWf.cons _ ih.1
+    -- · apply Core.GlobalWf.classDecl
+    --   · sorry
+    --   · sorry
+    --   · sorry
+    --   · sorry
+  · sorry
+--   cases wf; case _ wfh wftl =>
+--   replace wf := wf wfh
+--   cases wftl; case _ G G' x K n ms ms' j0 ms'def lk h1 h2 h3 =>
+--   have wkn_j0 : Elab (.cons (.classDecl x K Vect.nil) G) (.cons (.opent x K.translate) G') := by
+--     apply Elab.classDecl (x := x) (K := K) (ms := Vect.nil) (ms' := Vect.nil) j0; simp
+--   apply And.intro
+--   · simp;
+--     revert ms'; revert ms; intro ms; apply ms.induction
+--     case _ =>
+--       simp; intro ms'
+--       apply Core.ListGlobalWf.cons _ wf.1;
+--       apply Core.GlobalWf.opent
+--       apply Translation.ValidOpenKind.Sound h1
+--       apply Translation.GlobalEnv.lookup_none_sound x j0 lk
+--     case _ =>
+--       simp; intro n mthname mthTy ms ih1 ih2 ih3
+--       generalize mdef : (Vect.fold [] List.cons fun i =>
+--        Core.Global.openm ( Vect.cons (mthname, mthTy) ms i).fst ⟦(Vect.cons (mthname, mthTy) ms i).snd⟧) = ms' at *
+--       have lem :
+--         (Vect.fold [] List.cons fun i => Core.Global.openm (Vect.cons (mthname, mthTy) ms i).fst ⟦(Vect.cons (mthname, mthTy) ms i).snd⟧) =
+--           List.cons (Core.Global.openm mthname mthTy.translate) (Vect.fold [] List.cons (fun i => Core.Global.openm (ms i).fst ⟦(ms i).snd⟧)) := by sorry
 
-      sorry
-  sorry
+--     --   intro n hd tl wftl
+--     --   simp; apply Core.ListGlobalWf.cons _ wftl;
+
+--       sorry
+--   sorry
